%%%%%%%%%%%%%%%%%%%%%%%
\item
%%%%%%%%%%%%%%%%%%%%%%%

\begin{enumerate}[wide, labelindent = 0pt, label = (\alph*)]
	\item
	      We should first formally state what the problem is asking of us.
	      \begin{align*}
		      {(E + 1)}^k + {(E - 1)}^k
		       & = \sum_{i = 0}^k \binom{k}{i} E_i + \sum_{i = 0}^k {(-1)}^{k - i} \binom{k}{i} E_i \\
		       & = \sum_{i = 0}^k \left( 1 + {(-1)}^i \right) \binom{k}{i} E_i                      \\
		       & = 2 \sum_{i = 0}^{k / 2} \binom{k}{2i} E_{2i}
	      \end{align*}
	      Therefore, we need to show that
	      \[
		      \sum_{i = 0}^{l} \binom{2l}{2i} E_{2i} = 0
	      \]
	      for all integers $l$.
	      \begin{align*}
		      1
		       & = \sec z \cdot \cos z        \\
		       & = \left(
		      \sum_{n = 0}^\infty \frac{{(-1)}^n}{(2n)!} E_{2n} z^{2n}
		      \right) \cdot \left(
		      \sum_{n = 0}^\infty \frac{{(-1)}^n}{(2n)!} z^{2n}
		      \right)                         \\
		       & = \sum_{l = 0}^\infty \left(
		      \sum_{i = 0}^l \frac{{(-1)}^i}{(2i)!} E_{2i} \cdot \frac{{(-1)}^{2l - i}}{(k - 2i)!}
		      \right) z^{2l}                  \\
		       & = \sum_{l = 0}^\infty \left(
		      \frac{1}{(2l)!} \sum_{i = 0}^l \binom{2l}{2i} E_{2i}
		      \right) z^{2l}
	      \end{align*}
	      \[
		      \therefore (\forall l \geq 1) \sum_{i = 0}^l \binom{2l}{2i} E_{2i} = 0
	      \]

	      We could use this formula to determine successive terms of this sequence.
	      \[
		      l = 1:\; E_2 + E_0 = 0 \Rightarrow E_2 = -1
	      \]
	      \[
		      l = 2:\; E_4 + 6E_2 + E_0 = 0 \Rightarrow E_4 = 5
	      \]
	      \[
		      l = 3:\; E_6 + 15E_4 + 15E_2 + E_0 = 0 \Rightarrow E_6 = -61
	      \]
	      \[
		      l = 4:\; E_8 + 28E_6 + 70E_4 + 28E_2 + E_0 = 0 \Rightarrow E_9 = 1385
	      \]

	\item
	      It is sometimes a good idea to start with the more general formula then apply it to the more concrete problem,
	      as this could lead to less work.
	      \begin{align*}
		      \sec \pi x
		       & = \frac{4}{\pi} \sum_{i = 0}^\infty \frac{{(-1)}^i (2i + 1)}{{(2i + 1)}^2 - 4x^2}                     \\
		       & = \frac{4}{\pi} \sum_{i = 0}^\infty \frac{{(-1)}^i}{2i + 1} {\left(
			      1 - {\left( \frac{2x}{2i + 1} \right)}^2
		      \right)}^{-1}                                                                                            \\
		       & = \frac{4}{\pi} \sum_{i = 0}^\infty \frac{{(-1)}^i}{2i + 1} \sum_{n = 0}^\infty {\left(
			      \frac{2x}{2i + 1}
		      \right)}^{2n}                                                                                            \\
		       & = \frac{4}{\pi} \sum_{i = 0}^\infty \sum_{n = 0}^\infty {(-1)}^i \frac{4^n}{{2i + 1}^{2n + 1}} x^{2n} \\
		       & = \sum_{n = 0}^\infty \left(
		      \frac{4^{n + 1}}{\pi} \sum_{i = 0}^\infty \frac{{(-1)}^i}{{(2i + 1)}^{2n + 1}}
		      \right) x^{2n}                                                                                           \\
		       & = \sum_{n = 0}^\infty {(-1)}^n \frac{E_{2n}}{(2n)!} {(\pi x)}^{2n}
	      \end{align*}
	      We thus compare the last two series term-by-term to obtain
	      \[
		      \sum_{i = 0}^\infty \frac{{(-1)}^i}{{(2i + 1)}^{2n + 1}}
		      = \frac{\pi^{2n + 1} {(-1)}^n E_{2n}}{4^{n + 1} (2n)!}
	      \]
	      as the answer to part (b).

	      Substituting $n = 1$ for part (a), we get
	      \[
		      \sum_{i = 0}^\infty \frac{{(-1)}^i}{{(2i + 1)}^3}
		      = \frac{\pi^3 {(-1)}^1 E_{2}}{4^2 \cdot 2!}
		      = \frac{\pi^3}{32}.
	      \]
\end{enumerate}