%%%%%%%%%%%%%%%%%%%%%%%
\item
%%%%%%%%%%%%%%%%%%%%%%%

We want to evaluate
\[
	f(x) = \sum_{n = 0}^\infty \frac{{(-1)}^n {(n + 1)}^2 x^{2n + 1}}{(2n + 1)!}.
\]
To this end, we want to express ${(n + 1)}^2 = n^2 + 2n + 1$ in terms of $2n + 2$ and $(2n + 1)(2n + 3)$
as they can easily be obtained by differentiation.
We employ Horner's schema to do so.
\[
	\begin{array}{ c | c c c }
		             & 1 & 2                           & 1                      \\
		-1           &   & -1                          & -1                     \\
		\hline
		             & 1 & 1                           & \multicolumn{1}{|c}{0} \\
		-\frac{3}{2} &   & -\frac{3}{2}                &                        \\
		\hline
		             & 1 & \multicolumn{1}{|c}{-\half} &
	\end{array}
\]
\begin{align*}
	\Rightarrow n^2 + 2n + 1
	 & = \left( \left( n + \frac{3}{2} \right) - \half \right) (n + 1) \\
	 & = \frac{1}{4} (2n + 3) (2n + 2) - \frac{1}{4} (2n + 2)
\end{align*}
\begin{align*}
	\therefore f(x)
	 & = \frac{1}{4} \left(
	\sum_{n = 0}^\infty \frac{{(-1)}^n}{(2n + 1)!} (2n + 3) (2n + 2) x^{2n + 1}
	- \sum_{n = 0}^\infty \frac{{(-1)}^n}{(2n + 1)!} (2n + 2) x^{2n + 1}
	\right)                                                                                                        \\
	 & = \frac{1}{4} \frac{d^2}{dx^2} \left( \sum_{n = 0}^\infty \frac{{(-1)}^n}{(2n + 1)!} x^{2n + 3} \right)
	-\frac{1}{4} \frac{d}{dx} \left( \sum_{n = 0}^\infty \frac{{(-1)}^n}{(2n + 1)!} x^{2n + 2} \right)             \\
	 & = \frac{1}{4} \frac{d^2}{dx^2} \left( x^2 \sin x \right) - \frac{1}{4} \frac{d}{dx} \left( x \sin x \right) \\
	 & = \frac{1}{4} \left( 2\sin x + 4x\cos x - x^2 \sin x \right) - \frac{1}{4} \left( \sin x + x \cos x \right) \\
	 & = \frac{1 - x^2}{4} \sin x + \frac{3}{4} x \cos x
\end{align*}