%%%%%%%%%%%%%%%%%%%%%%%
\item
%%%%%%%%%%%%%%%%%%%%%%%

Half of the challenge of this problem is expressing the $n$th term in closed form.
Let us denote the first term as $a_1$.
\begin{align*}
	a_n
	&= \cfrac{
		\left( \prod_{j = 1}^{n - 1} \frac{2j - 1}{2} \right) \cdot {\left( \frac{2n - 1}{2} \right)}^2
	}{
		(2n + 7) (2n + 5) {(2n + 3)}^2 n!
	} \\
	&= \frac{(2n - 1)!! (2n - 1)}{2^{n + 1} (2n + 7) (2n + 5) {(2n + 3)}^2 n!} \\
	&= \cfrac{\cfrac{(2n)!}{2^n n!} \cdot (2n - 1)}{2^{n + 1} (2n + 7) (2n + 5) {(2n + 3)}^2 n!} \\
	&= \frac{(2n - 1) \cdot (2n)!}{2^{2n + 1} (2n + 7) (2n + 5) (2n + 3) {(n!)}^2}
\end{align*}
\begin{align*}
	\Rightarrow \frac{a_{n + 1}}{a_n}
	&= \frac{{(2n + 1)}^2 (2n + 2) {(2n + 3)}^2}{(2n + 9) (2n + 5) {(n + 1)}^2 (2n - 1)} \\
	&\xrightarrow{n \rightarrow \infty} 4 > 1
\end{align*}
Therefore, the given series diverges.