%%%%%%%%%%%%%%%%%%%%%%%
\item
%%%%%%%%%%%%%%%%%%%%%%%

\begin{align*}
	f(\theta)
	 & = \sum_{n = 0}^\infty \frac{\sin \left(n + 1\right) \theta}{2n + 1}                                                                                                   \\
	 & = \Im \left\{ \sum_{n = 0}^\infty \frac{1}{2n + 1} e^{i (n + 1) \theta} \right\}                                                                                      \\
	 & = \Im \left\{ e^{i \frac{\theta}{2}} \sum_{n = 0}^\infty \frac{1}{2n + 1} {\left( e^{i \frac{\theta}{2}} \right)}^{2n + 1} \right\}                                   \\
	 & = \Im \left\{ e^{i \frac{\theta}{2}} \tanh^{-1} \left( e^{i \frac{\theta}{2}} \right) \right\}                                                                        \\
	 & = \half \Im \left\{ e^{i \frac{\theta}{2}} \ln \left( \frac{1 + e^{i \frac{\theta}{2}}}{1 - e^{i \frac{\theta}{2}}} \right) \right\}                                  \\
	 & = \half \Im \left\{ e^{i \frac{\theta}{2}} \ln \left( i \cot \frac{\theta}{4} \right) \right\}                                                                        \\
	 & = \half \Im \left\{ \left( \cos \frac{\theta}{2} + i \sin \frac{\theta}{2} \right) \left( \ln \left( \cot \frac{\theta}{4} \right) + i \frac{\pi}{2} \right) \right\} \\
	 & = \frac{\pi}{4} \cos \frac{\theta}{2} + \half \ln \left( \cot \frac{\theta}{4} \right) \sin \frac{\theta}{2}
\end{align*}
