%%%%%%%%%%%%%%%%%%%%%%%
\item
%%%%%%%%%%%%%%%%%%%%%%%
For very large $x$,
\[
	y'' \approx \frac{y}{4}
	\Rightarrow y \approx e^{\pm \frac{x}{2}}.
\]
Thus, for $y$ to vanish at infinity, we must have $y \approx e^{-x / 2}$.
As $y$ must also vanish at the origin, let us write $y = f(x) x e^{-x / 2}$ with $f(x)$ regular everywhere.
\[
	y' = \left( \frac{f'}{f} + \frac{1}{x} - \half \right) y
\]
\begin{align*}
	\Rightarrow y''
	 & = \left( \frac{f''}{f} - {\left( \frac{f'}{f} \right)}^2 - \frac{1}{x^2} \right) y
	+ {\left( \frac{f'}{f} + \frac{1}{x} - \half \right)}^2 y                                                     \\
	 & = \left( \frac{f''}{f} + \left( \frac{2}{x} - 1 \right) \frac{f'}{f} - \frac{1}{x} + \frac{1}{4} \right) y
\end{align*}
\[
	\Rightarrow \frac{f''}{f} + \left( \frac{2}{x} - 1 \right) \frac{f'}{f} - \frac{K + 1}{x} = 0
\]

Let us write $f(x) = \sum_{n=0}^\infty a_n x^n$.
Substitution and tedious algebra yield
\[
	2a_1 - (K + 1) a_0 + \sum_{n=1}^\infty ((n + 1)(n + 2)a_{n + 1} - (n + K + 1) a_n) x^n = 0
\]
\[
	\Rightarrow (\forall n)\; (n + 1)(n + 2)a_{n + 1} = (n + K + 1) a_n.
\]
If $\{a_n\}$ never terminated, this would mean that $a_n \approx \frac{1}{n!}$ for large values of $n$,
leading to $f(x) \approx e^x$ and $y$ diverging to infinity as $x$ increases.
\[
	\therefore K_n = -n\; (n = 1, 2, 3, \dots)
\]