%%%%%%%%%%%%%%%%%%%%%%%
\item
%%%%%%%%%%%%%%%%%%%%%%%

Notice how $(x(1 - x))' = 1 - 2x$.
\begin{align*}
	0
	&= x(1 - x) y'' + 4y' + 2y \\
	&= x(1 - x) y'' + (x(1 - x))' y' + (2x + 3) y' + 2y \\
	&= (x(1 - x)y')' + ((2x + 3)y)'
\end{align*}
\[
	\Rightarrow x(1 - x)y' + (2x + 3)y = A
\]

Let us define the integrating factor $\lambda$:
\begin{align*}
	\lambda
	&= \exp \left( \int dx \frac{2x + 3}{x(1 - x)} \right) \\
	&= \exp \left( \int dx \left( \frac{3}{x} - \frac{5}{x - 1} \right) \right) \\
	&= \exp \left( 3 \ln x - 5 \ln (x - 1) \right) \\
	&= \frac{x^3}{{(x - 1)}^5}
\end{align*}
\[
	\Rightarrow (\lambda y)' = \frac{A}{x(1 - x)} \cdot \lambda = \frac{Ax^2}{{(x - 1)}^6}
\]
\begin{align*}
	\Rightarrow \lambda y
	&= \int dx \frac{Ax^2}{{(x - 1)}^6} \\
	&= A \int dx \left( \frac{1}{{(x - 1)}^4} + \frac{2}{{(x - 1)}^5} + \frac{1}{{(x - 1)}^6} \right) \\
	&= -A \frac{10x^2 - 5x + 1}{30 {(x - 1)}^5} + C_2
\end{align*}
\[
	\therefore y = C_1 \frac{10x^2 - 5x + 1}{x^3} + C_2 \frac{{(1 - x)}^5}{x^3}
\]