%%%%%%%%%%%%%%%%%%%%%%%
\item
%%%%%%%%%%%%%%%%%%%%%%%

\[
	\frac{y''}{{(1 + y'^2)}^{3/2}} = \pm \frac{1}{a}
	\Rightarrow \frac{y'}{\sqrt{1 + y'^2}} = \pm \frac{x + C_1}{a}
\]
\[
	\Rightarrow y'^2 = {\left( \frac{x + C_1}{a} \right)}^2 (1 + y'^2)
	\Rightarrow y' = \pm \frac{{\left( \frac{x + C_1}{a} \right)}^2}{\sqrt{1 - {\left( \frac{x + C_1}{a} \right)}^2}}
\]
\[
	\therefore y = \pm \half \left( a \sin^{-1} \left( \frac{x + C_1}{a} \right) - (x + C_1) \sqrt{1 - {\left( \frac{x + C_1}{a} \right)}^2}\right) + C_2
\]