%%%%%%%%%%%%%%%%%%%%%%%
\item
%%%%%%%%%%%%%%%%%%%%%%%

\[
	y' y'' = e^y y'
	\Rightarrow \int dy' y' = \int dy e^y
	\Rightarrow \half y'^2 = e^y + C_1
\]
\[
	\Rightarrow \frac{dy}{\sqrt{e^y + C_1}} = \sqrt{2} dx
\]
Basic calculus yields
\[
	\int \frac{dy}{\sqrt{e^y + C_1}}
	= \frac{1}{\sqrt{C_1}} \ln \left( \frac{\sqrt{e^y + C_1} - \sqrt{A}}{\sqrt{e^y + C_1} + \sqrt{C_1}} \right) + A.
\]
\[
	\therefore \ln \left( \frac{\sqrt{e^y + C_1} - \sqrt{C_1}}{\sqrt{e^y + C_1} + \sqrt{C_1}} \right) = \sqrt{2C_1}x + C_2
\]