%%%%%%%%%%%%%%%%%%%%%%%
\item
%%%%%%%%%%%%%%%%%%%%%%%

\begin{enumerate}[wide, labelindent = 0pt, label = (\alph*)]
\item
The Fourier transform of the input function is given by
\begin{align*}
    \Tilde{f}(\omega)
    &= \int_{-\infty}^\infty \frac{d\omega}{\sqrt{2\pi}} f(t) e^{-i\omega t} \\
    &= \inv{\sqrt{2\pi}} \int_0^\infty dt e^{-(\lambda + i\omega) t} \\
    &= \inv{\sqrt{2\pi}} \inv{\lambda + i\omega}
\end{align*}
while that of the response function is given by
\begin{align*}
    \Tilde{F}(\omega)
    &= \int_{-\infty}^\infty \frac{d\omega}{\sqrt{2\pi}} F(t) e^{-i\omega t} \\
    &= \inv{\sqrt{2\pi}} \int_0^\infty dt \left(
        e^{-(\lambda + i\omega)t} - e^{-(\lambda + \alpha + i\omega)t}
    \right) \\
    & = \inv{\sqrt{2\pi}} \left(
        \inv{\lambda + i\omega} - \inv{\lambda + \alpha + i\omega}
    \right).
\end{align*}
Meanwhile, since the system is linear, we know that
\[
    \Tilde{F}(\omega) = G(-\omega) \Tilde{f}(\omega)
\]
since each oscillatory mode $e^{i\omega t}$ transforms to $G(-\omega) e^{-i\omega t}$.
\[
    \therefore G(\omega) = 1 + \frac{\lambda - i\omega}{\lambda + \alpha - i\omega}
\]

\item
\begin{align*}
    \Tilde{f}(\omega)
    &= \int_{-\infty}^\infty \frac{dt}{\sqrt{2\pi}} A \delta(x) e^{-i\omega t} \\
    &= \frac{A}{\sqrt{2\pi}}
\end{align*}
\begin{align*}
    \Rightarrow \Tilde{F}(\omega)
    &= G(-\omega) \Tilde{f}(\omega) \\
    &= \frac{A}{\sqrt{2\pi}} \left(1 + \frac{\lambda - i\omega}{\lambda + \alpha - i\omega} \right) \\
    &= \frac{A}{\sqrt{2\pi}} \left(2 - \frac{\alpha}{\lambda + \alpha - i\omega} \right)
\end{align*}
\[
    \therefore F(t)
    = A \left( 2\delta(t) - \alpha e^{-(\lambda + \alpha + i\omega)t} \right)
\]

\end{enumerate}