%%%%%%%%%%%%%%%%%%%%%%%
\item
%%%%%%%%%%%%%%%%%%%%%%%

\begin{enumerate}[wide, labelindent = 0pt, label = (\alph*)]
\item
We basically express the piecewise function
\[
    f(x) = \begin{cases}
        -e^{x} & (-1 < x < 0) \\
        e^{-x} & ( 0 < x < 1) \\
    \end{cases}
\]
as a Fourier series.
Since this function is defined to be odd, we will only obtain the sine terms:
\[
    f(x) = \sum_{n=1}^\infty B_n \sin n\pi x.
\]
\[
    \Rightarrow B_n
    = 2\int_0^1 dx e^{-x} \sin n\pi x 
    = \frac{2n\pi}{n^2 \pi^2 + 1} \left( 1 - \frac{{(-1)}^n}{e} \right)
\]
\begin{align*}
    \therefore f(x)
    &= \sum_{n=1}^\infty \frac{2\pi n}{n^2 \pi^2 + 1} \left( 1 - \frac{{(-1)}^n}{e} \right) \sin n\pi x \\
    &= \frac{ \pi}{ \pi^2 + 1} \left( 1 + \inv{e} \right) \sin  \pi x
     + \frac{2\pi}{4\pi^2 + 1} \left( 1 - \inv{e} \right) \sin 2\pi x \\
    &\quad + \frac{3\pi}{9\pi^2 + 1} \left( 1 - \inv{e} \right) \sin 3\pi x
     + \cdots
\end{align*}

\item
Let
\[
    f(x)
    = e^{-x}
    = \frac{A_0}{2} + \sum_{n=1}^\infty \left( A_n \cos 2n\pi x + B_n \sin 2n\pi x \right)
    \quad (0 < x < 1).
\]
\[
    \Rightarrow A_n
    = 2 \int_0^1 dx e^{-x} \cos 2n\pi x
    = \frac{2}{4n^2 \pi^2 + 1} \left( 1 - \inv{e} \right)
\]
\[
    B_n
    = 2 \int_0^1 dx e^{-x} \sin 2n\pi x
    = \frac{4n\pi}{4n^2 \pi^2 + 1} \left( 1 - \inv{e} \right)
\]
\begin{align*}
    \therefore f(x)
    &= \left( 1 - \inv{e} \right) \left(
        1 + \sum_{n=1}^\infty \frac{2\cos 2n\pi x + 4n\pi\sin 2n\pi}{4n^2 \pi^2 + 1}
    \right) \\
    &= \left( 1 - \inv{e} \right) \left(
        1
        + \frac{2\cos 2\pi x + 4\pi\sin 2\pi x}{4\pi^2 + 1} \right. \\
    &\quad\left. + \frac{2\cos 4\pi x + 8\pi\sin 4\pi x}{16\pi^2 + 1}
        + \frac{2\cos 6\pi x + 12\pi\sin 6\pi x}{36\pi^2 + 1}
        + \cdots
    \right)
\end{align*}

\end{enumerate}