%%%%%%%%%%%%%%%%%%%%%%%
\item
%%%%%%%%%%%%%%%%%%%%%%%

Equalities between delta ``function''-like things should be dealt with care.
A rigorous-enough definition of equality for physicists is given by
\[
    A(x) = B(x) \Leftrightarrow
    \left( \forall f(x) \right) \int dx f(x) A(x) = \int dx f(x) B(x).
\]
Hence, this problem could be viewed as proving the equality
\[
    \delta\left[ g(x) \right] = \frac{\delta(x - x_0)}{\abs{g'(x_0)}}.
\]
\begin{align*}
    \int_a^b dx f(x) \delta\left[ g(x) \right]
    &= \int_{g(a)}^{g(b)} \frac{du}{g'(x(u))} f(x(u)) \delta(u) && (u := g(x)) \\
    &= \evalAt{ \sign\left( g(b) - g(a) \right) \frac{f(x(u))}{g'(x(u))} }{u = 0} \\
    &= \sign\left( g'(x_0) \right) \frac{f(x_0)}{g'(x_0)} \\
    &= \frac{f(x_0)}{\abs{g'(x_0)}}
\end{align*}