%%%%%%%%%%%%%%%%%%%%%%%
\item
%%%%%%%%%%%%%%%%%%%%%%%

\begin{enumerate}[wide, labelindent = 0pt, label = (Solution \arabic*)]
\item
We perform a partial fraction decomposition to obtain formulae
whose inverse Laplace transforms are trivial (or at least well documented).
\[
    \inv{\left( s^2 + 1 \right) (s - 1)}
    = \frac{-s/2 - 1/2}{s^2 + 1} + \frac{1/2}{s - 1}
    = \half \left( \inv{s - 1} - \frac{s}{s^2 + 1} - \inv{s^2 +1} \right)
\]
\[
    \therefore \invLapltransf{\inv{\left( s^2 + 1 \right) (s - 1)}}(x)
    = \half \left( e^x - \cos x - \sin x \right)
\]

\item
We apply properties of Laplace transforms to gradually reduce the problem.
\begin{align*}
    \invLapltransf{\inv{\left( s^2 + 1 \right) (s - 1)}}(x)
    &= e^x \invLapltransf{\inv{\left( {(s + 1)}^2 + 1 \right) s}}(x) \\
    &= e^x \int_0^x dt \invLapltransf{\inv{{(s + 1)}^2 + 1}}(t) \\
    &= e^x \int_0^x dt e^{-t} \invLapltransf{\inv{s^2 + 1}(t)} \\
    &= e^x \int_0^x dt e^{-t} \sin t \\
    &= \half \left( e^x - \cos x - \sin x \right)
\end{align*}

\end{enumerate}