%%%%%%%%%%%%%%%%%%%%%%%
\item
%%%%%%%%%%%%%%%%%%%%%%%

\begin{enumerate}[wide, labelindent = 0pt, label = (\alph*)]
\item
\begin{align*}
    {\left( \Tilde{(AB)} \right)}_{ij}
    &= {\left(BA\right)}_{ji} \\
    &= \sum_k B_{jk} A_{ki} \\
    &= \sum_k {\left( \Tilde{A} \right)}_{ik} {\left( \Tilde{B} \right)}_{kj} \\
    &= {\left( \Tilde{A} \Tilde{B} \right)}_{ij}
\end{align*}
\[
    \therefore \Tilde{(AB)} = \Tilde{B} \Tilde{A}
\]

\item
\begin{align*}
    {\left( {(AB)}^\dagger \right)}_{ij}
    &= {\left( {(AB)}_{ji} \right)}^* \\
    &= {\left( \sum_k A_{jk} B_{ki} \right)}^* \\
    &= \sum_k {B_{ki}}^* {A_{jk}}^* \\
    &= \sum_k {\left( B^\dagger \right)}_{ik} {\left( A^\dagger \right)}_{kj} \\
    &= {\left( B^\dagger A^\dagger \right)}_{ij}
\end{align*}
\[
    \therefore {(AB)}^\dagger = B^\dagger A^\dagger
\]

\item
\begin{align*}
    {(A (BC))}_{ij}
    &= \sum_k A_{ik} {(BC)}_{kj} \\
    &= \sum_k \sum_l A_{ik} B_{kl} C_{lj} \\
    &= \sum_l {(AB)}_{il} C_{lj} \\
    &= {((AB) C)}_{ij}
\end{align*}
\[
    \therefore A(BC) = (AB)C
\]

\item
\begin{align*}
    \Tr ABC
    &= \sum_i {(ABC)}_{ii} \\
    &= \sum_i \sum_j A_{ij} {(BC)}_{ji} \\
    &= \sum_i \sum_j \sum_k A_{ij} B_{jk} C_{ki} \\
    &= \sum_j \sum_k B_{jk} {(CA)}_{kj} \\
    &= \sum_j {(BCA)}_{jj} \\
    &= \Tr BCA
\end{align*}

\end{enumerate}
