%%%%%%%%%%%%%%%%%%%%%%%
\item
%%%%%%%%%%%%%%%%%%%%%%%

\begin{enumerate}[wide, labelindent = 0pt, label = (\alph*)]
\item
\begin{align*}
    x_1^\dagger x_1
    &= x_1^\dagger 1 x_1 \\
    &= x_1^\dagger U^\dagger U x_1 \\
    &= {(U x_1)}^\dagger (U x_1) \\
    &= {(\lambda_1 x_1)}^\dagger (\lambda_1 x_1) \\
    &= {\abs{\lambda_1}}^2 x_1^\dagger x_1
\end{align*}
Since $x_1$ is nonzero, we therefore obtain
\[
    \abs{\lambda_1}^2 = 1
    \Leftrightarrow \abs{\lambda_1} = 1.
\]

\item
\begin{align*}
    x_1^\dagger x_2
    &= x_1^\dagger 1 x_2 \\
    &= x_1^\dagger U^\dagger U x_2 \\
    &= {(U x_1)}^\dagger (U x_2) \\
    &= {(\lambda_1 x_1)}^\dagger (\lambda_2 x_2) \\
    &= \lambda_1^* \lambda_2 x_1^\dagger x_2
\end{align*}
By part~(a), $\lambda_1 \neq \lambda_2$ implies $\lambda_1^* \lambda_2 \neq 1$.
\[
    \therefore x_1^\dagger x_2 = 0
\]

\end{enumerate}
