%%%%%%%%%%%%%%%%%%%%%%%                                                          
\item
%%%%%%%%%%%%%%%%%%%%%%%

Let $z := e^{i\theta}$.
\[
	dz = ie^{i\theta} d\theta,\;
	\cos\theta = \half\left( z + \inv{z} \right),\;
	\sin^2 \theta = \frac{1 - \cos 2\theta}{2} = \inv{4}\left( 2 - z^2 - \inv{z^2} \right)
\]
\begin{align*}
	I
    &:= \int_0^{2\pi} d\theta \frac{\sin^2 \theta}{a + b\cos\theta} \\
    &= \half \oint_{\abs{z} = 1} \frac{
        -{\left( z^2 - 1 \right)}^2
    }{
        z \left( bz^2 + 2az + b \right)
    }
\end{align*}
Let $f(z)$ be the integrand here.
$f(z)$ has simple poles at
\[
    0,\; z^*_\pm := \frac{-a \pm \sqrt{a^2 - b^2}}{b},
\]
among which $0$ and $z^*_+$ lie within the unit circle (which is our contour).

\begin{align*}
    \therefore I
    &= \half \cdot 2i\pi \left( \res{z = 0} f(z) + \res{z = z^*_+} f(z) \right) \\
    &= i\pi \left(
        \evalAt{
            \frac{-{\left( z^2 - 1 \right)}^2}{bz^2 + 2az + b}
        }{z = 0} + \evalAt{ 
            \frac{-{\left( z^2 - 1 \right)}^2}{z \left( bz + a + \sqrt{a^2 - b^2} \right)}
        }{z = z^*_+}
    \right) \\
    &= \frac{i\pi}{b} \left(
        -1 + 4\frac{
            a^4 + b^4 - 2ab\left( (a-b)\sqrt{a^2 - b^2} + b^2 \right)
        }{
            -a + \sqrt{a^2 - b^2}
        }
    \right)
\end{align*}
