%%%%%%%%%%%%%%%%%%%%%%%
\item
%%%%%%%%%%%%%%%%%%%%%%%

Let us integrate $f(x) := \frac{e^{iaz}}{{\left( 1 + z^2 \right)}^2}$, again along \reffig{}~\ref{fig:problem3-3,4}.
\begin{align*}
	\oint_C dz f(z)
	= 2i\pi \res{z = i} f(z)
	= 2i\pi \cdot \evalAt{\frac{d}{dz} \frac{e^{iaz}}{{\left( z + i \right)}^2}}{z = i}
	= \frac{\pi}{2} (a + 1) e^{-a}
\end{align*}
and
\begin{align*}
	\oint_C dx f(z)
	 & = \int_{-R}^{R} dx \frac{e^{iax}}{{\left( 1 + x^2 \right)}^2}
	+\int_0^{\pi} d\theta iRe^{i\theta} \frac{e^{iaRe^{i\theta}}}{{\left( 1 + R^2 e^{2i\theta} \right)}^2}       \\
	 & \xrightarrow{R \rightarrow \infty} \int_{-\infty}^{\infty} dx \frac{e^{iax}}{{\left( 1 + x^2 \right)}^2}.
\end{align*}
\begin{align*}
	\therefore \int_{0}^{\infty} dx \frac{\cos ax}{{\left( 1 + x^2 \right)}^2}
	 & = \half \int_{-\infty}^{\infty} dx \frac{\cos ax}{{\left( 1 + x^2 \right)}^2}                            \\
	 & = \half \cdot \Re \left\{ \int_{-\infty}^{\infty} dx \frac{e^{iax}}{{\left( 1 + x^2 \right)}^2} \right\} \\
	 & = \frac{\pi}{4} (a + 1) e^{-a}
\end{align*}