%%%%%%%%%%%%%%%%%%%%%%%
\item
%%%%%%%%%%%%%%%%%%%%%%%

\begin{enumerate}[wide, labelindent = 0pt, label = (\alph*)]
\item
\[
    \Gamma\left( \half \right)
    = \sqrt{{\Gamma\left( \half \right)}^2}
    = \sqrt{\frac{\pi}{\sin \halfpi}}
    = \sqrt{\pi}
\]

\item
\[
    \Gamma\left( \frac{5}{2} \right)
    = \frac{3}{2} \Gamma\left( \frac{3}{2} \right)
    = \frac{3}{4} \Gamma\left( \half \right)
    = \frac{3\sqrt{\pi}}{4}
\]

\item
\[
    \Beta(1, 3)
    = \frac{\Gamma(1) \Gamma(3)}{\Gamma(4)}
    = \frac{0! 2!}{3!}
    = \frac{1}{3}
\]

\item
\[
    \Beta \left( \half, -\half \right)
    = \frac{\Gamma\left( \half \right) \Gamma\left( -\half \right)}{\Gamma\left( 0 \right)}
    = \frac{\sqrt{\pi} \cdot \frac{\sqrt{\pi}}{-1/2}}{\infty}
    = 0
\]

\item
\[
    \Gamma\left( \frac{1}{3} \right) \Gamma\left( -\frac{1}{3} \right)
    = -3 \Gamma\left( \frac{1}{3} \right) \Gamma\left( \frac{2}{3} \right)
    = -3 \cdot \frac{\pi}{\sin \frac{\pi}{3}}
    = -2\sqrt{3}\pi
\]

\end{enumerate}