%%%%%%%%%%%%%%%%%%%%%%%
\item
%%%%%%%%%%%%%%%%%%%%%%%

\[
    -\Ei(-x)
    = \int_{-\infty}^{-x} dy \frac{e^y}{y}
    = \int_\infty^x dt \frac{e^{-t}}{t}
\]
\begin{align*}
    \therefore \int_0^\infty dx e^{-ax} \left( -\Ei(-x) \right)
    &= \int_0^\infty dx \int_{\infty}^x dt \frac{e^{-ax - t}}{t} \\
    &= -\int_0^\infty dx \int_{-(a + 1)x}^\infty du \frac{e^{-u}}{u - ax} && (u := ax + t) \\
    &= -\int_0^\infty du \int_0^{u / (a + 1)} dx \frac{e^{-u}}{u - ax} \\ 
    &= -\int_0^\infty du \int_0^{1/a(a + 1)} dv \frac{u}{a} \frac{e^{-u}}{u(1 - v)} && (v := \frac{ax}{u}) \\
    &= -\inv{a} \int_0^\infty du e^{-u} \cdot \int_0^{1/a(a + 1)} \frac{dv}{1 - v} \\
    &= \inv{a} \ln\left( 1 - \inv{a(a + 1)} \right)
\end{align*}